Launchbury/FutureCardinality.thy
@@ -3,17 +3,17 @@ imports CallFutures CardinalityAnalysis Cardinality-Domain-Lists
 begin
 
 locale FutureAnalysis =
- fixes Fexp :: "exp \<Rightarrow> Arity \<rightarrow> future set"
+ fixes Texp :: "exp \<Rightarrow> Arity \<rightarrow> future set"
 begin
 
 fun FBinds :: "heap \<Rightarrow> AEnv \<rightarrow> (var \<Rightarrow> future set)"
   where "FBinds [] = (\<Lambda> ae. \<bottom>)"
-      | "FBinds ((x,e)#\<Gamma>) = (\<Lambda> ae. (\<lambda> x'. (if x' = x then fup\<cdot>(Fexp e)\<cdot>(ae x) else (FBinds \<Gamma>\<cdot>ae) x)))"
+      | "FBinds ((x,e)#\<Gamma>) = (\<Lambda> ae. (\<lambda> x'. (if x' = x then fup\<cdot>(Texp e)\<cdot>(ae x) else (FBinds \<Gamma>\<cdot>ae) x)))"
 
 lemma FBinds_Nil_simp[simp]: "FBinds []\<cdot>ae = \<bottom>" by simp
 
 lemma FBinds_Cons[simp]:
-  "FBinds ((x,e)#\<Gamma>)\<cdot>ae = (\<lambda> x'. (if x' = x then fup\<cdot>(Fexp e)\<cdot>(ae x) else (FBinds \<Gamma>\<cdot>ae) x))" by simp
+  "FBinds ((x,e)#\<Gamma>)\<cdot>ae = (\<lambda> x'. (if x' = x then fup\<cdot>(Texp e)\<cdot>(ae x) else (FBinds \<Gamma>\<cdot>ae) x))" by simp
 
 lemmas FBinds.simps[simp del]
 
@@ -36,13 +36,13 @@ fun Fstack :: "stack \<Rightarrow> future set"
   | "Fstack (Dummy x # S) = Fstack S"
 
 fun prognosis :: "AEnv \<Rightarrow> Arity \<Rightarrow> conf \<Rightarrow> var \<Rightarrow> two"
-   where "prognosis ae a (\<Gamma>, e, S) = pathsCard (paths (FBinds \<Gamma>\<cdot>ae) (future_add (Fexp e\<cdot>a) (Fstack S)))"
+   where "prognosis ae a (\<Gamma>, e, S) = pathsCard (paths (FBinds \<Gamma>\<cdot>ae) (future_add (Texp e\<cdot>a) (Fstack S)))"
 end
 
 locale FutureAnalysisCorrect = FutureAnalysis +
-  assumes Fexp_App: "Fexp (App e x)\<cdot>a = may_call x ((Fexp e)\<cdot>(inc\<cdot>a))"
-  assumes Fexp_Lam: "without y ` (Fexp e \<cdot>(pred\<cdot>n)) = Fexp (Lam [y]. e) \<cdot> n"
-  assumes Fexp_subst: "Fexp (e[y::=x])\<cdot>a = may_call x (without y ` ((Fexp e)\<cdot>a))"
+  assumes Texp_App: "Texp (App e x)\<cdot>a = may_call x ((Texp e)\<cdot>(inc\<cdot>a))"
+  assumes Texp_Lam: "without y ` (Texp e \<cdot>(pred\<cdot>n)) = Texp (Lam [y]. e) \<cdot> n"
+  assumes Texp_subst: "Texp (e[y::=x])\<cdot>a = may_call x (without y ` ((Texp e)\<cdot>a))"
 begin
 
   sublocale CardinalityPrognosisCorrect prognosis
@@ -59,9 +59,9 @@ begin
       assume "x \<in> ap S"
       hence "\<exists> f \<in> Fstack S. f x > 1"
         by(induction S rule: Fstack.induct)(auto simp add: may_call_multiple_calls)
-      hence "\<exists> f \<in> future_add (Fexp e\<cdot>a) (Fstack S). f x > 1"
+      hence "\<exists> f \<in> future_add (Texp e\<cdot>a) (Fstack S). f x > 1"
         using future_add_subset2 by auto
-      hence "[x,x] \<in> paths (FBinds \<Gamma>\<cdot>ae) (future_add (Fexp e\<cdot>a) (Fstack S))" 
+      hence "[x,x] \<in> paths (FBinds \<Gamma>\<cdot>ae) (future_add (Texp e\<cdot>a) (Fstack S))" 
         apply -
         apply (erule bexE)
         apply (rule paths_intros)
@@ -73,7 +73,7 @@ begin
         apply (simp add: possible_def after_def)
         apply rule
         done
-      hence "pathCard [x,x] x \<sqsubseteq> pathsCard (paths (FBinds \<Gamma>\<cdot>ae) (future_add (Fexp e\<cdot>a) (Fstack S))) x"
+      hence "pathCard [x,x] x \<sqsubseteq> pathsCard (paths (FBinds \<Gamma>\<cdot>ae) (future_add (Texp e\<cdot>a) (Fstack S))) x"
         by (metis fun_belowD paths_Card_above)
       also have "pathCard [x,x] x = many" by (auto simp add: pathCard_def)
       finally
@@ -82,17 +82,17 @@ begin
     qed
   next
     fix ae a \<Gamma> e x S
-    have "future_add (Fexp e\<cdot>(inc\<cdot>a)) (may_call x (Fstack S)) = future_add (may_call x (Fexp e\<cdot>(inc\<cdot>a))) (Fstack S)"
+    have "future_add (Texp e\<cdot>(inc\<cdot>a)) (may_call x (Fstack S)) = future_add (may_call x (Texp e\<cdot>(inc\<cdot>a))) (Fstack S)"
       by (rule future_add_may_call_twist)
-    hence "(future_add (Fexp e\<cdot>(inc\<cdot>a)) (may_call x (Fstack S))) = future_add (Fexp (App e x)\<cdot>a) (Fstack S)"
-      by (simp add: Fexp_App)
+    hence "(future_add (Texp e\<cdot>(inc\<cdot>a)) (may_call x (Fstack S))) = future_add (Texp (App e x)\<cdot>a) (Fstack S)"
+      by (simp add: Texp_App)
     thus "prognosis ae (inc\<cdot>a) (\<Gamma>, e, Arg x # S) \<sqsubseteq> prognosis ae a (\<Gamma>, App e x, S)"
       by simp
   next
     fix ae a \<Gamma> e y x S
-    have "Fexp e[y::=x]\<cdot>(pred\<cdot>a) = may_call x (Fexp (Lam [y]. e)\<cdot>a)" 
-      by (simp add: Fexp_Lam Fexp_subst)
-    hence "future_add (Fexp e[y::=x]\<cdot>(pred\<cdot>a)) (Fstack S) = future_add (Fexp (Lam [y]. e)\<cdot>a) (may_call x (Fstack S))"
+    have "Texp e[y::=x]\<cdot>(pred\<cdot>a) = may_call x (Texp (Lam [y]. e)\<cdot>a)" 
+      by (simp add: Texp_Lam Texp_subst)
+    hence "future_add (Texp e[y::=x]\<cdot>(pred\<cdot>a)) (Fstack S) = future_add (Texp (Lam [y]. e)\<cdot>a) (may_call x (Fstack S))"
       by (metis future_add_may_call_twist)
     thus "prognosis ae (pred\<cdot>a) (\<Gamma>, e[y::=x], S) \<sqsubseteq> prognosis ae a (\<Gamma>, Lam [y]. e, Arg x # S)"
       by simp
@@ -102,20 +102,20 @@ begin
     assume "ae x = up\<cdot>u"
     assume "a \<sqsubseteq> u"
 
-    have "paths (FBinds (delete x \<Gamma>)\<cdot>ae) (future_add (Fexp e\<cdot>u) (Fstack S)) \<subseteq> {tl p |p. p \<in> paths (FBinds \<Gamma>\<cdot>ae) (future_add (Fexp (Var x)\<cdot>a) (Fstack S)) \<and> hd p = x}"
+    have "paths (FBinds (delete x \<Gamma>)\<cdot>ae) (future_add (Texp e\<cdot>u) (Fstack S)) \<subseteq> {tl p |p. p \<in> paths (FBinds \<Gamma>\<cdot>ae) (future_add (Texp (Var x)\<cdot>a) (Fstack S)) \<and> hd p = x}"
     proof
       fix p 
-      assume "p \<in> paths (FBinds (delete x \<Gamma>)\<cdot>ae) (future_add (Fexp e\<cdot>u) (Fstack S))"
+      assume "p \<in> paths (FBinds (delete x \<Gamma>)\<cdot>ae) (future_add (Texp e\<cdot>u) (Fstack S))"
 
-      have "x# p \<in>paths (FBinds \<Gamma>\<cdot>ae) (future_add (Fexp (Var x)\<cdot>a) (Fstack S))"
+      have "x# p \<in>paths (FBinds \<Gamma>\<cdot>ae) (future_add (Texp (Var x)\<cdot>a) (Fstack S))"
       proof
         
       qed
-      thus "p \<in> {tl p |p. p \<in> paths (FBinds \<Gamma>\<cdot>ae) (future_add (Fexp (Var x)\<cdot>a) (Fstack S)) \<and> hd p = x}" by force
+      thus "p \<in> {tl p |p. p \<in> paths (FBinds \<Gamma>\<cdot>ae) (future_add (Texp (Var x)\<cdot>a) (Fstack S)) \<and> hd p = x}" by force
     qed
-    hence "pathsCard (paths (FBinds (delete x \<Gamma>)\<cdot>ae) (future_add (Fexp e\<cdot>u) (Fstack S))) \<sqsubseteq> pathsCard {tl p |p. p \<in> paths (FBinds \<Gamma>\<cdot>ae) (future_add (Fexp (Var x)\<cdot>a) (Fstack S)) \<and> hd p = x}"
+    hence "pathsCard (paths (FBinds (delete x \<Gamma>)\<cdot>ae) (future_add (Texp e\<cdot>u) (Fstack S))) \<sqsubseteq> pathsCard {tl p |p. p \<in> paths (FBinds \<Gamma>\<cdot>ae) (future_add (Texp (Var x)\<cdot>a) (Fstack S)) \<and> hd p = x}"
       by (rule pathsCard_mono)
-    hence "pathsCard (paths (FBinds (delete x \<Gamma>)\<cdot>ae) (future_add (Fexp e\<cdot>u) (Fstack S))) \<sqsubseteq> record_call x\<cdot>(pathsCard (paths (FBinds \<Gamma>\<cdot>ae) (future_add (Fexp (Var x)\<cdot>a) (Fstack S))))"
+    hence "pathsCard (paths (FBinds (delete x \<Gamma>)\<cdot>ae) (future_add (Texp e\<cdot>u) (Fstack S))) \<sqsubseteq> record_call x\<cdot>(pathsCard (paths (FBinds \<Gamma>\<cdot>ae) (future_add (Texp (Var x)\<cdot>a) (Fstack S))))"
       by (rule below_trans[OF _ record_call_pathsCard])
     thus "prognosis ae u (delete x \<Gamma>, e, Upd x # S) \<sqsubseteq> record_call x\<cdot>(prognosis ae a (\<Gamma>, Var x, S))" by simp
   oops
