Launchbury/TTreeImplCardinalitySafe.thy
@@ -25,7 +25,7 @@ begin
        (auto simp add: empty_is_bottom[symmetric] carrier_Fexp dest!: set_mp[OF Aexp_edom])
 
   lemma carrier_FBinds: "carrier ((FBinds \<Gamma>\<cdot>ae) x) \<subseteq> fv \<Gamma>"
-  apply (simp add: Fexp.AnalBinds_lookup)
+  apply (simp add: Texp.AnalBinds_lookup)
   apply (auto split: option.split simp add: empty_is_bottom[symmetric] )
   apply (case_tac "ae x")
   apply (auto simp add: empty_is_bottom[symmetric] carrier_Fexp dest!: set_mp[OF Aexp_edom])
@@ -39,7 +39,7 @@ begin
   proof
     fix \<Gamma> :: heap and ae ae' :: AEnv and u e S as
     assume "ae f|` domA \<Gamma> = ae' f|` domA \<Gamma>"
-    from Fexp.AnalBinds_cong[OF this]
+    from Texp.AnalBinds_cong[OF this]
     show "prognosis ae as u (\<Gamma>, e, S) = prognosis ae' as u (\<Gamma>, e, S)" by simp
   next
     fix ae as a \<Gamma> e S
@@ -50,11 +50,11 @@ begin
       hence "[x,x] \<in> paths (Fstack as S)"
         by (induction S rule: Fstack.induct)
            (auto 4 4 intro: set_mp[OF both_contains_arg1] set_mp[OF both_contains_arg2] paths_Cons_nxt)
-      hence "[x,x] \<in> paths (Fexp e\<cdot>a \<otimes>\<otimes> Fstack as S)"
+      hence "[x,x] \<in> paths (Texp e\<cdot>a \<otimes>\<otimes> Fstack as S)"
         by (rule set_mp[OF both_contains_arg2])
-      hence "[x,x] \<in> paths (substitute (FBinds \<Gamma>\<cdot>ae) (thunks \<Gamma>) (Fexp e\<cdot>a \<otimes>\<otimes> Fstack as S))" 
+      hence "[x,x] \<in> paths (substitute (FBinds \<Gamma>\<cdot>ae) (thunks \<Gamma>) (Texp e\<cdot>a \<otimes>\<otimes> Fstack as S))" 
         by (rule set_mp[OF substitute_contains_arg])
-      hence "pathCard [x,x] x \<sqsubseteq> pathsCard (paths (substitute (FBinds \<Gamma>\<cdot>ae) (thunks \<Gamma>) (Fexp e\<cdot>a \<otimes>\<otimes> Fstack as S))) x"
+      hence "pathCard [x,x] x \<sqsubseteq> pathsCard (paths (substitute (FBinds \<Gamma>\<cdot>ae) (thunks \<Gamma>) (Texp e\<cdot>a \<otimes>\<otimes> Fstack as S))) x"
         by (metis fun_belowD paths_Card_above)
       also have "pathCard [x,x] x = many"  by (auto simp add: pathCard_def)
       finally
@@ -64,7 +64,7 @@ begin
   next
     fix \<Gamma> \<Delta> :: heap and e :: exp and ae :: AEnv and as u S
     assume "map_of \<Gamma> = map_of \<Delta>"
-    hence "FBinds \<Gamma> = FBinds \<Delta>" and "thunks \<Gamma> = thunks \<Delta>" by (auto intro!: cfun_eqI  thunks_cong simp add: Fexp.AnalBinds_lookup)
+    hence "FBinds \<Gamma> = FBinds \<Delta>" and "thunks \<Gamma> = thunks \<Delta>" by (auto intro!: cfun_eqI  thunks_cong simp add: Texp.AnalBinds_lookup)
     thus "prognosis ae as u (\<Gamma>, e, S) = prognosis ae as u (\<Delta>, e, S)"  by simp
   next
     fix \<Gamma> :: heap and e :: exp and ae :: AEnv and as u S x
@@ -73,9 +73,9 @@ begin
   fix \<Gamma> :: heap and e :: exp and ae :: AEnv and as a S x
   assume "ae x = \<bottom>"
 
-  hence "FBinds (delete x \<Gamma>)\<cdot>ae = FBinds \<Gamma>\<cdot>ae" by (rule Fexp.AnalBinds_delete_bot)
+  hence "FBinds (delete x \<Gamma>)\<cdot>ae = FBinds \<Gamma>\<cdot>ae" by (rule Texp.AnalBinds_delete_bot)
   moreover
-  hence "((FBinds \<Gamma>\<cdot>ae) x) = \<bottom>" by (metis Fexp.AnalBinds_delete_lookup)
+  hence "((FBinds \<Gamma>\<cdot>ae) x) = \<bottom>" by (metis Texp.AnalBinds_delete_lookup)
   ultimately
   show "prognosis ae as a (\<Gamma>, e, S) \<sqsubseteq> prognosis ae as a (delete x \<Gamma>, e, S)"
     by (simp add: substitute_T_delete empty_is_bottom)
@@ -85,9 +85,9 @@ begin
     also have "pathCard [x] \<sqsubseteq> pathsCard ({[],[x]})"
       by (rule paths_Card_above) simp
     also have "\<dots> = pathsCard (paths (single x))" by simp
-    also have "single x \<sqsubseteq> (Fexp (Var x)\<cdot>a)" by (rule Fexp_Var)
-    also have "\<dots> \<sqsubseteq> Fexp (Var x)\<cdot>a \<otimes>\<otimes> Fstack as S" by (rule both_above_arg1)
-    also have "\<dots> \<sqsubseteq> substitute  (FBinds \<Gamma>\<cdot>ae) (thunks \<Gamma>) (Fexp (Var x)\<cdot>a \<otimes>\<otimes> Fstack as S)" by (rule substitute_above_arg)
+    also have "single x \<sqsubseteq> (Texp (Var x)\<cdot>a)" by (rule Texp_Var)
+    also have "\<dots> \<sqsubseteq> Texp (Var x)\<cdot>a \<otimes>\<otimes> Fstack as S" by (rule both_above_arg1)
+    also have "\<dots> \<sqsubseteq> substitute  (FBinds \<Gamma>\<cdot>ae) (thunks \<Gamma>) (Texp (Var x)\<cdot>a \<otimes>\<otimes> Fstack as S)" by (rule substitute_above_arg)
     also have "pathsCard (paths \<dots>) x = prognosis ae as a (\<Gamma>, Var x, S) x" by simp
     finally
     show "once \<sqsubseteq> prognosis ae as a (\<Gamma>, Var x, S) x"
@@ -97,18 +97,18 @@ begin
   sublocale CardinalityPrognosisApp prognosis
   proof default
     fix ae as a \<Gamma> e x S
-    have "Fexp e\<cdot>(inc\<cdot>a)  \<otimes>\<otimes> many_calls x \<otimes>\<otimes> Fstack as S = many_calls x  \<otimes>\<otimes> (Fexp e)\<cdot>(inc\<cdot>a) \<otimes>\<otimes> Fstack as S"
+    have "Texp e\<cdot>(inc\<cdot>a)  \<otimes>\<otimes> many_calls x \<otimes>\<otimes> Fstack as S = many_calls x  \<otimes>\<otimes> (Texp e)\<cdot>(inc\<cdot>a) \<otimes>\<otimes> Fstack as S"
       by (metis both_assoc both_comm)
     thus "prognosis ae as (inc\<cdot>a) (\<Gamma>, e, Arg x # S) \<sqsubseteq> prognosis ae as a (\<Gamma>, App e x, S)"
-      by simp (intro pathsCard_mono' paths_mono substitute_mono2' both_mono1' Fexp_App)
+      by simp (intro pathsCard_mono' paths_mono substitute_mono2' both_mono1' Texp_App)
   qed
 
   sublocale CardinalityPrognosisLam prognosis
   proof default
     fix ae as a \<Gamma> e y x S
-    have "Fexp e[y::=x]\<cdot>(pred\<cdot>a) \<sqsubseteq> many_calls x  \<otimes>\<otimes> Fexp (Lam [y]. e)\<cdot>a"
-      by (rule below_trans[OF Fexp_subst both_mono2'[OF Fexp_Lam]])
-    moreover have "Fexp (Lam [y]. e)\<cdot>a \<otimes>\<otimes> many_calls x \<otimes>\<otimes> Fstack as S = many_calls x  \<otimes>\<otimes> Fexp (Lam [y]. e)\<cdot>a \<otimes>\<otimes> Fstack as S"
+    have "Texp e[y::=x]\<cdot>(pred\<cdot>a) \<sqsubseteq> many_calls x  \<otimes>\<otimes> Texp (Lam [y]. e)\<cdot>a"
+      by (rule below_trans[OF Texp_subst both_mono2'[OF Texp_Lam]])
+    moreover have "Texp (Lam [y]. e)\<cdot>a \<otimes>\<otimes> many_calls x \<otimes>\<otimes> Fstack as S = many_calls x  \<otimes>\<otimes> Texp (Lam [y]. e)\<cdot>a \<otimes>\<otimes> Fstack as S"
       by (metis both_assoc both_comm)
     ultimately  
     show "prognosis ae as (pred\<cdot>a) (\<Gamma>, e[y::=x], S) \<sqsubseteq> prognosis ae as a (\<Gamma>, Lam [y]. e, Arg x # S)"
@@ -125,20 +125,20 @@ begin
     hence "x \<notin> thunks \<Gamma>" using `map_of \<Gamma> x = Some e` by (metis thunksE)
     hence [simp]: "f_nxt (FBinds \<Gamma>\<cdot>ae) (thunks \<Gamma>) x = FBinds \<Gamma>\<cdot>ae" by (auto simp add: f_nxt_def)
 
-    have "prognosis ae as u (\<Gamma>, e, S) = pathsCard (paths (substitute (FBinds \<Gamma>\<cdot>ae) (thunks \<Gamma>) (Fexp e\<cdot>u \<otimes>\<otimes> Fstack as S)))"
+    have "prognosis ae as u (\<Gamma>, e, S) = pathsCard (paths (substitute (FBinds \<Gamma>\<cdot>ae) (thunks \<Gamma>) (Texp e\<cdot>u \<otimes>\<otimes> Fstack as S)))"
       by simp
-    also have "\<dots> = pathsCard (paths (substitute (FBinds \<Gamma>\<cdot>ae) (thunks \<Gamma>) (nxt (single x) x \<otimes>\<otimes> Fexp e\<cdot>u  \<otimes>\<otimes> Fstack as S)))"
+    also have "\<dots> = pathsCard (paths (substitute (FBinds \<Gamma>\<cdot>ae) (thunks \<Gamma>) (nxt (single x) x \<otimes>\<otimes> Texp e\<cdot>u  \<otimes>\<otimes> Fstack as S)))"
       by simp
-    also have "\<dots> = pathsCard (paths (substitute (FBinds \<Gamma>\<cdot>ae) (thunks \<Gamma>) ((nxt (single x) x \<otimes>\<otimes> Fstack as S) \<otimes>\<otimes> Fexp e\<cdot>u )))"
+    also have "\<dots> = pathsCard (paths (substitute (FBinds \<Gamma>\<cdot>ae) (thunks \<Gamma>) ((nxt (single x) x \<otimes>\<otimes> Fstack as S) \<otimes>\<otimes> Texp e\<cdot>u )))"
       by (metis both_assoc both_comm)
-    also have "\<dots> \<sqsubseteq> pathsCard (paths (substitute (FBinds \<Gamma>\<cdot>ae) (thunks \<Gamma>) (nxt (single x \<otimes>\<otimes> Fstack as S) x \<otimes>\<otimes> Fexp e\<cdot>u)))"
+    also have "\<dots> \<sqsubseteq> pathsCard (paths (substitute (FBinds \<Gamma>\<cdot>ae) (thunks \<Gamma>) (nxt (single x \<otimes>\<otimes> Fstack as S) x \<otimes>\<otimes> Texp e\<cdot>u)))"
       by (intro pathsCard_mono' paths_mono substitute_mono2' both_mono1'  nxt_both_left) simp
     also have "\<dots> = pathsCard (paths (nxt (substitute (FBinds \<Gamma>\<cdot>ae) (thunks \<Gamma>) (single x \<otimes>\<otimes> Fstack as S)) x))"
-      using `map_of \<Gamma> x = Some e` `ae x = up\<cdot>u` by (simp add: Fexp.AnalBinds_lookup)
+      using `map_of \<Gamma> x = Some e` `ae x = up\<cdot>u` by (simp add: Texp.AnalBinds_lookup)
     also have "\<dots> \<sqsubseteq> record_call x \<cdot>(pathsCard (paths (substitute (FBinds \<Gamma>\<cdot>ae) (thunks \<Gamma>) (single x \<otimes>\<otimes> Fstack as S))))"
       by (rule pathsCard_paths_nxt)
-    also have "\<dots> \<sqsubseteq> record_call x \<cdot>(pathsCard (paths (substitute (FBinds \<Gamma>\<cdot>ae) (thunks \<Gamma>) ((Fexp (Var x)\<cdot>a) \<otimes>\<otimes> Fstack as S))))"
-      by (intro monofun_cfun_arg pathsCard_mono' paths_mono substitute_mono2' both_mono1' Fexp_Var)
+    also have "\<dots> \<sqsubseteq> record_call x \<cdot>(pathsCard (paths (substitute (FBinds \<Gamma>\<cdot>ae) (thunks \<Gamma>) ((Texp (Var x)\<cdot>a) \<otimes>\<otimes> Fstack as S))))"
+      by (intro monofun_cfun_arg pathsCard_mono' paths_mono substitute_mono2' both_mono1' Texp_Var)
     also have "\<dots> = record_call x \<cdot>(prognosis ae as a (\<Gamma>, Var x, S))"
       by simp
     finally
@@ -150,24 +150,24 @@ begin
     assume "\<not> isVal e"
     hence "x \<in> thunks \<Gamma>" using `map_of \<Gamma> x = Some e` by (metis thunksI)
     hence [simp]: "f_nxt (FBinds \<Gamma>\<cdot>ae) (thunks \<Gamma>) x = FBinds (delete x \<Gamma>)\<cdot>ae" 
-      by (auto simp add: f_nxt_def Fexp.AnalBinds_delete_to_fun_upd empty_is_bottom)
+      by (auto simp add: f_nxt_def Texp.AnalBinds_delete_to_fun_upd empty_is_bottom)
 
-    have "prognosis ae as u (delete x \<Gamma>, e, Upd x # S) = pathsCard (paths (substitute (FBinds (delete x \<Gamma>)\<cdot>ae) (thunks (delete x \<Gamma>)) (Fexp e\<cdot>u \<otimes>\<otimes> Fstack as S)))"
+    have "prognosis ae as u (delete x \<Gamma>, e, Upd x # S) = pathsCard (paths (substitute (FBinds (delete x \<Gamma>)\<cdot>ae) (thunks (delete x \<Gamma>)) (Texp e\<cdot>u \<otimes>\<otimes> Fstack as S)))"
       by simp
-    also have "\<dots> = pathsCard (paths (substitute (FBinds (delete x \<Gamma>)\<cdot>ae) (thunks \<Gamma>) (Fexp e\<cdot>u \<otimes>\<otimes> Fstack as S)))"
+    also have "\<dots> = pathsCard (paths (substitute (FBinds (delete x \<Gamma>)\<cdot>ae) (thunks \<Gamma>) (Texp e\<cdot>u \<otimes>\<otimes> Fstack as S)))"
        by (rule arg_cong[OF substitute_cong_T]) (auto simp add: empty_is_bottom)
-    also have "\<dots> = pathsCard (paths (substitute (FBinds (delete x \<Gamma>)\<cdot>ae) (thunks \<Gamma>) (nxt (single x) x \<otimes>\<otimes> Fexp e\<cdot>u  \<otimes>\<otimes> Fstack as S)))"
+    also have "\<dots> = pathsCard (paths (substitute (FBinds (delete x \<Gamma>)\<cdot>ae) (thunks \<Gamma>) (nxt (single x) x \<otimes>\<otimes> Texp e\<cdot>u  \<otimes>\<otimes> Fstack as S)))"
       by simp
-    also have "\<dots> = pathsCard (paths (substitute (FBinds (delete x \<Gamma>)\<cdot>ae) (thunks \<Gamma>) ((nxt (single x) x \<otimes>\<otimes> Fstack as S) \<otimes>\<otimes> Fexp e\<cdot>u )))"
+    also have "\<dots> = pathsCard (paths (substitute (FBinds (delete x \<Gamma>)\<cdot>ae) (thunks \<Gamma>) ((nxt (single x) x \<otimes>\<otimes> Fstack as S) \<otimes>\<otimes> Texp e\<cdot>u )))"
       by (metis both_assoc both_comm)
-    also have "\<dots> \<sqsubseteq> pathsCard (paths (substitute (FBinds (delete x \<Gamma>)\<cdot>ae) (thunks \<Gamma>) (nxt (single x \<otimes>\<otimes> Fstack as S) x  \<otimes>\<otimes> Fexp e\<cdot>u)))"
+    also have "\<dots> \<sqsubseteq> pathsCard (paths (substitute (FBinds (delete x \<Gamma>)\<cdot>ae) (thunks \<Gamma>) (nxt (single x \<otimes>\<otimes> Fstack as S) x  \<otimes>\<otimes> Texp e\<cdot>u)))"
       by (intro pathsCard_mono' paths_mono substitute_mono2' both_mono1'  nxt_both_left) simp
     also have "\<dots> = pathsCard (paths (nxt (substitute (FBinds \<Gamma>\<cdot>ae) (thunks \<Gamma>) (single x \<otimes>\<otimes> Fstack as S)) x))"
-      using `map_of \<Gamma> x = Some e` `ae x = up\<cdot>u` by (simp add: Fexp.AnalBinds_lookup)
+      using `map_of \<Gamma> x = Some e` `ae x = up\<cdot>u` by (simp add: Texp.AnalBinds_lookup)
     also have "\<dots> \<sqsubseteq> record_call x \<cdot>(pathsCard (paths (substitute (FBinds \<Gamma>\<cdot>ae) (thunks \<Gamma>) (single x \<otimes>\<otimes> Fstack as S))))"
       by (rule pathsCard_paths_nxt)
-    also have "\<dots> \<sqsubseteq> record_call x \<cdot>(pathsCard (paths (substitute (FBinds \<Gamma>\<cdot>ae) (thunks \<Gamma>) ((Fexp (Var x)\<cdot>a) \<otimes>\<otimes> Fstack as S))))"
-      by (intro monofun_cfun_arg pathsCard_mono' paths_mono substitute_mono2' both_mono1' Fexp_Var)
+    also have "\<dots> \<sqsubseteq> record_call x \<cdot>(pathsCard (paths (substitute (FBinds \<Gamma>\<cdot>ae) (thunks \<Gamma>) ((Texp (Var x)\<cdot>a) \<otimes>\<otimes> Fstack as S))))"
+      by (intro monofun_cfun_arg pathsCard_mono' paths_mono substitute_mono2' both_mono1' Texp_Var)
     also have "\<dots> = record_call x \<cdot>(prognosis ae as a (\<Gamma>, Var x, S))"
       by simp
     finally
@@ -175,7 +175,7 @@ begin
   next
     fix \<Gamma> :: heap and e :: exp and ae :: AEnv and  x :: var and as S
     assume "isVal e"
-    hence "repeatable (Fexp e\<cdot>0)" by (rule Fun_repeatable)
+    hence "repeatable (Texp e\<cdot>0)" by (rule Fun_repeatable)
 
     assume [simp]: "x \<notin> domA \<Gamma>"
 
@@ -183,13 +183,13 @@ begin
       using `isVal e`
       by (auto simp add: thunks_Cons dest: set_mp[OF thunks_domA])
 
-    have "fup\<cdot>(Fexp e)\<cdot>(ae x) \<sqsubseteq> Fexp e\<cdot>0" by (metis fup2 monofun_cfun_arg up_zero_top)
-    hence "substitute ((FBinds \<Gamma>\<cdot>ae)(x := fup\<cdot>(Fexp e)\<cdot>(ae x))) (thunks \<Gamma>) (Fexp e\<cdot>0 \<otimes>\<otimes> Fstack as S) \<sqsubseteq> substitute ((FBinds \<Gamma>\<cdot>ae)(x := Fexp e\<cdot>0)) (thunks \<Gamma>) (Fexp e\<cdot>0 \<otimes>\<otimes> Fstack as S)"
+    have "fup\<cdot>(Texp e)\<cdot>(ae x) \<sqsubseteq> Texp e\<cdot>0" by (metis fup2 monofun_cfun_arg up_zero_top)
+    hence "substitute ((FBinds \<Gamma>\<cdot>ae)(x := fup\<cdot>(Texp e)\<cdot>(ae x))) (thunks \<Gamma>) (Texp e\<cdot>0 \<otimes>\<otimes> Fstack as S) \<sqsubseteq> substitute ((FBinds \<Gamma>\<cdot>ae)(x := Texp e\<cdot>0)) (thunks \<Gamma>) (Texp e\<cdot>0 \<otimes>\<otimes> Fstack as S)"
       by (intro substitute_mono1' fun_upd_mono below_refl monofun_cfun_arg)
-    also have "\<dots> = substitute (((FBinds \<Gamma>\<cdot>ae)(x := Fexp e\<cdot>0))(x := empty)) (thunks \<Gamma>) (Fexp e\<cdot>0 \<otimes>\<otimes> Fstack as S)"
-      using `repeatable (Fexp e\<cdot>0)` by (rule substitute_remove_anyways, simp)
-    also have "((FBinds \<Gamma>\<cdot>ae)(x := Fexp e\<cdot>0))(x := empty) = FBinds \<Gamma>\<cdot>ae"
-      by (simp add: fun_upd_idem Fexp.AnalBinds_not_there empty_is_bottom)
+    also have "\<dots> = substitute (((FBinds \<Gamma>\<cdot>ae)(x := Texp e\<cdot>0))(x := empty)) (thunks \<Gamma>) (Texp e\<cdot>0 \<otimes>\<otimes> Fstack as S)"
+      using `repeatable (Texp e\<cdot>0)` by (rule substitute_remove_anyways, simp)
+    also have "((FBinds \<Gamma>\<cdot>ae)(x := Texp e\<cdot>0))(x := empty) = FBinds \<Gamma>\<cdot>ae"
+      by (simp add: fun_upd_idem Texp.AnalBinds_not_there empty_is_bottom)
     finally
     show "prognosis ae as 0 ((x, e) # \<Gamma>, e, S) \<sqsubseteq> prognosis ae as 0 (\<Gamma>, e, Upd x # S)"
       by (simp, intro pathsCard_mono' paths_mono)
@@ -198,17 +198,17 @@ begin
   sublocale CardinalityPrognosisIfThenElse prognosis
   proof default
     fix ae as \<Gamma> scrut e1 e2 S a
-    have "Fexp scrut\<cdot>0 \<otimes>\<otimes> (Fexp e1\<cdot>a \<oplus>\<oplus> Fexp e2\<cdot>a) \<sqsubseteq> Fexp (scrut ? e1 : e2)\<cdot>a"
-      by (rule Fexp_IfThenElse)
-    hence "substitute (FBinds \<Gamma>\<cdot>ae) (thunks \<Gamma>) (Fexp scrut\<cdot>0 \<otimes>\<otimes> (Fexp e1\<cdot>a \<oplus>\<oplus> Fexp e2\<cdot>a) \<otimes>\<otimes> Fstack as S) \<sqsubseteq> substitute (FBinds \<Gamma>\<cdot>ae) (thunks \<Gamma>) (Fexp (scrut ? e1 : e2)\<cdot>a \<otimes>\<otimes> Fstack as S)"
+    have "Texp scrut\<cdot>0 \<otimes>\<otimes> (Texp e1\<cdot>a \<oplus>\<oplus> Texp e2\<cdot>a) \<sqsubseteq> Texp (scrut ? e1 : e2)\<cdot>a"
+      by (rule Texp_IfThenElse)
+    hence "substitute (FBinds \<Gamma>\<cdot>ae) (thunks \<Gamma>) (Texp scrut\<cdot>0 \<otimes>\<otimes> (Texp e1\<cdot>a \<oplus>\<oplus> Texp e2\<cdot>a) \<otimes>\<otimes> Fstack as S) \<sqsubseteq> substitute (FBinds \<Gamma>\<cdot>ae) (thunks \<Gamma>) (Texp (scrut ? e1 : e2)\<cdot>a \<otimes>\<otimes> Fstack as S)"
       by (rule substitute_mono2'[OF both_mono1'])
     thus "prognosis ae (a#as) 0 (\<Gamma>, scrut, Alts e1 e2 # S) \<sqsubseteq> prognosis ae as a (\<Gamma>, scrut ? e1 : e2, S)"
       by (simp, intro pathsCard_mono' paths_mono)
   next
     fix ae as a \<Gamma> b e1 e2 S
-    have "Fexp (if b then e1 else e2)\<cdot>a \<sqsubseteq> Fexp e1\<cdot>a \<oplus>\<oplus> Fexp e2\<cdot>a"
+    have "Texp (if b then e1 else e2)\<cdot>a \<sqsubseteq> Texp e1\<cdot>a \<oplus>\<oplus> Texp e2\<cdot>a"
       by (auto simp add: either_above_arg1 either_above_arg2)
-    hence "substitute (FBinds \<Gamma>\<cdot>ae) (thunks \<Gamma>) (Fexp (if b then e1 else e2)\<cdot>a \<otimes>\<otimes> Fstack as S) \<sqsubseteq> substitute (FBinds \<Gamma>\<cdot>ae) (thunks \<Gamma>) (Fexp (Bool b)\<cdot>0 \<otimes>\<otimes> (Fexp e1\<cdot>a \<oplus>\<oplus> Fexp e2\<cdot>a) \<otimes>\<otimes> Fstack as S)"
+    hence "substitute (FBinds \<Gamma>\<cdot>ae) (thunks \<Gamma>) (Texp (if b then e1 else e2)\<cdot>a \<otimes>\<otimes> Fstack as S) \<sqsubseteq> substitute (FBinds \<Gamma>\<cdot>ae) (thunks \<Gamma>) (Texp (Bool b)\<cdot>0 \<otimes>\<otimes> (Texp e1\<cdot>a \<oplus>\<oplus> Texp e2\<cdot>a) \<otimes>\<otimes> Fstack as S)"
       by (rule substitute_mono2'[OF both_mono1'[OF below_trans[OF _ both_above_arg2]]])
     thus "prognosis ae as a (\<Gamma>, if b then e1 else e2, S) \<sqsubseteq> prognosis ae (a#as) 0 (\<Gamma>, Bool b, Alts e1 e2 # S)"
       by (auto intro!: pathsCard_mono' paths_mono)
@@ -220,9 +220,9 @@ context TTreeAnalysisCardinalityHeap
 begin
 
   definition cHeap where
-    "cHeap \<Gamma> e = (\<Lambda> a. pathsCard (paths (Fheap \<Gamma> e\<cdot>a)))"
+    "cHeap \<Gamma> e = (\<Lambda> a. pathsCard (paths (Theap \<Gamma> e\<cdot>a)))"
 
-  lemma cHeap_simp: "(cHeap \<Gamma> e)\<cdot>a = pathsCard (paths (Fheap \<Gamma> e\<cdot>a))"
+  lemma cHeap_simp: "(cHeap \<Gamma> e)\<cdot>a = pathsCard (paths (Theap \<Gamma> e\<cdot>a))"
     unfolding cHeap_def  by (rule beta_cfun) (intro cont2cont)
   
   sublocale CardinalityHeap cHeap.
@@ -233,12 +233,12 @@ begin
     assume "x \<in> thunks \<Gamma>"
     moreover
     assume "many \<sqsubseteq> (cHeap \<Gamma> e\<cdot>a) x"
-    hence "many \<sqsubseteq> pathsCard (paths (Fheap \<Gamma> e \<cdot>a)) x" unfolding cHeap_def by simp
-    hence "\<exists>p\<in> (paths (Fheap \<Gamma> e\<cdot>a)). \<not> (one_call_in_path x p)" unfolding pathsCard_def
+    hence "many \<sqsubseteq> pathsCard (paths (Theap \<Gamma> e \<cdot>a)) x" unfolding cHeap_def by simp
+    hence "\<exists>p\<in> (paths (Theap \<Gamma> e\<cdot>a)). \<not> (one_call_in_path x p)" unfolding pathsCard_def
       by (auto split: if_splits)
     ultimately
     show "(Aheap \<Gamma> e\<cdot>a) x = up\<cdot>0"
-      by (metis Fheap_thunk)
+      by (metis Theap_thunk)
   next
     fix \<Gamma> e a
     show "edom (cHeap \<Gamma> e\<cdot>a) = edom (Aheap \<Gamma> e\<cdot>a)"
@@ -269,14 +269,14 @@ begin
 
     have const_on1:  "\<And> x. const_on (FBinds \<Delta>\<cdot>(Aheap \<Delta> e\<cdot>a)) (carrier ((FBinds \<Gamma>\<cdot>ae) x)) empty"
       unfolding const_on_edom_disj using fresh_distinct_fv[OF `atom \` domA \<Delta> \<sharp>* \<Gamma>`]
-      by (auto dest!: set_mp[OF carrier_FBinds] set_mp[OF Fexp.edom_AnalBinds])
+      by (auto dest!: set_mp[OF carrier_FBinds] set_mp[OF Texp.edom_AnalBinds])
     have const_on2:  "const_on (FBinds \<Delta>\<cdot>(Aheap \<Delta> e\<cdot>a)) (carrier (Fstack as S)) empty"
       unfolding const_on_edom_disj using fresh_distinct_fv[OF `atom \` domA \<Delta> \<sharp>* S`]
-      by (auto dest!: set_mp[OF carrier_FBinds] set_mp[OF carrier_Fstack] set_mp[OF Fexp.edom_AnalBinds] set_mp[OF ap_fv_subset ])
+      by (auto dest!: set_mp[OF carrier_FBinds] set_mp[OF carrier_Fstack] set_mp[OF Texp.edom_AnalBinds] set_mp[OF ap_fv_subset ])
     have  const_on3: "const_on (FBinds \<Gamma>\<cdot>ae) (- (- domA \<Delta>)) TTree.empty"
       and const_on4: "const_on (FBinds \<Delta>\<cdot>(Aheap \<Delta> e\<cdot>a)) (domA \<Gamma>) TTree.empty"
       unfolding const_on_edom_disj using fresh_distinct[OF `atom \` domA \<Delta> \<sharp>* \<Gamma>`]
-      by (auto dest!:  set_mp[OF Fexp.edom_AnalBinds])
+      by (auto dest!:  set_mp[OF Texp.edom_AnalBinds])
 
     have disj1: "\<And> x. carrier ((FBinds \<Gamma>\<cdot>ae) x) \<inter> domA \<Delta> = {}"
       using fresh_distinct_fv[OF `atom \` domA \<Delta> \<sharp>* \<Gamma>`]
@@ -297,7 +297,7 @@ begin
       have "ae x = \<bottom>" using True `domA \<Delta> \<inter> edom ae = {}` by auto
       ultimately
       show ?thesis using True 
-          by (auto simp add: Fexp.AnalBinds_lookup empty_is_bottom[symmetric] cong: option.case_cong)
+          by (auto simp add: Texp.AnalBinds_lookup empty_is_bottom[symmetric] cong: option.case_cong)
     next
       case False
       have "map_of \<Delta> x = None" using False by (metis domA_def map_of_eq_None_iff)
@@ -305,14 +305,14 @@ begin
       have "(Aheap \<Delta> e\<cdot>a) x = \<bottom>" using False using edom_Aheap by (metis contra_subsetD edomIff)
       ultimately
       show ?thesis using False
-         by (auto simp add: Fexp.AnalBinds_lookup empty_is_bottom[symmetric] cong: option.case_cong)
+         by (auto simp add: Texp.AnalBinds_lookup empty_is_bottom[symmetric] cong: option.case_cong)
     qed
     }
     note FBinds = ext[OF this]
     
     {
-    have "pathsCard (paths (substitute (FBinds (\<Delta> @ \<Gamma>)\<cdot>(Aheap \<Delta> e\<cdot>a \<squnion> ae)) (thunks (\<Delta> @ \<Gamma>)) (Fexp e\<cdot>a \<otimes>\<otimes> Fstack as S)))
-      = pathsCard (paths (substitute (FBinds \<Gamma>\<cdot>ae) (thunks (\<Delta> @ \<Gamma>)) (substitute (FBinds \<Delta>\<cdot>(Aheap \<Delta> e\<cdot>a))  (thunks (\<Delta> @ \<Gamma>))  (Fexp e\<cdot>a \<otimes>\<otimes> Fstack as S))))"
+    have "pathsCard (paths (substitute (FBinds (\<Delta> @ \<Gamma>)\<cdot>(Aheap \<Delta> e\<cdot>a \<squnion> ae)) (thunks (\<Delta> @ \<Gamma>)) (Texp e\<cdot>a \<otimes>\<otimes> Fstack as S)))
+      = pathsCard (paths (substitute (FBinds \<Gamma>\<cdot>ae) (thunks (\<Delta> @ \<Gamma>)) (substitute (FBinds \<Delta>\<cdot>(Aheap \<Delta> e\<cdot>a))  (thunks (\<Delta> @ \<Gamma>))  (Texp e\<cdot>a \<otimes>\<otimes> Fstack as S))))"
        by (simp add: substitute_substitute[OF const_on1] FBinds)
     also have "substitute (FBinds \<Gamma>\<cdot>ae) (thunks (\<Delta> @ \<Gamma>)) = substitute (FBinds \<Gamma>\<cdot>ae) (thunks \<Gamma>)"
       apply (rule substitute_cong_T)
@@ -322,7 +322,7 @@ begin
       apply (rule substitute_cong_T)
       using const_on4
       by (auto dest: set_mp[OF thunks_domA])
-    also have "substitute (FBinds \<Delta>\<cdot>(Aheap \<Delta> e\<cdot>a)) (thunks \<Delta>) (Fexp e\<cdot>a \<otimes>\<otimes> Fstack as S) = substitute (FBinds \<Delta>\<cdot>(Aheap \<Delta> e\<cdot>a)) (thunks \<Delta>) (Fexp e\<cdot>a) \<otimes>\<otimes> Fstack as S"
+    also have "substitute (FBinds \<Delta>\<cdot>(Aheap \<Delta> e\<cdot>a)) (thunks \<Delta>) (Texp e\<cdot>a \<otimes>\<otimes> Fstack as S) = substitute (FBinds \<Delta>\<cdot>(Aheap \<Delta> e\<cdot>a)) (thunks \<Delta>) (Texp e\<cdot>a) \<otimes>\<otimes> Fstack as S"
       by (rule substitute_only_empty_both[OF const_on2])
     also note calculation
     }
@@ -330,16 +330,16 @@ begin
     also
     note env_restr_split[where S = "domA \<Delta>"]
     also
-    have "pathsCard (paths (substitute (FBinds \<Gamma>\<cdot>ae) (thunks \<Gamma>) (substitute (FBinds \<Delta>\<cdot>(Aheap \<Delta> e\<cdot>a)) (thunks \<Delta>) (Fexp e\<cdot>a) \<otimes>\<otimes> Fstack as S))) f|` domA \<Delta> 
-        = pathsCard (paths (ftree_restr (domA \<Delta>) (substitute (FBinds \<Delta>\<cdot>(Aheap \<Delta> e\<cdot>a)) (thunks \<Delta>) (Fexp e\<cdot>a))))"
-          by (simp add: filter_paths_conv_free_restr ftree_restr_both ftree_rest_substitute[OF disj1]  ftree_restr_is_empty[OF disj2])
+    have "pathsCard (paths (substitute (FBinds \<Gamma>\<cdot>ae) (thunks \<Gamma>) (substitute (FBinds \<Delta>\<cdot>(Aheap \<Delta> e\<cdot>a)) (thunks \<Delta>) (Texp e\<cdot>a) \<otimes>\<otimes> Fstack as S))) f|` domA \<Delta> 
+        = pathsCard (paths (ttree_restr (domA \<Delta>) (substitute (FBinds \<Delta>\<cdot>(Aheap \<Delta> e\<cdot>a)) (thunks \<Delta>) (Texp e\<cdot>a))))"
+          by (simp add: filter_paths_conv_free_restr ttree_restr_both ttree_rest_substitute[OF disj1]  ttree_restr_is_empty[OF disj2])
     also
-    have "ftree_restr (domA \<Delta>) (substitute (FBinds \<Delta>\<cdot>(Aheap \<Delta> e\<cdot>a)) (thunks \<Delta>) (Fexp e\<cdot>a)) \<sqsubseteq> Fheap \<Delta> e\<cdot>a"  by (rule Fheap_substitute)
+    have "ttree_restr (domA \<Delta>) (substitute (FBinds \<Delta>\<cdot>(Aheap \<Delta> e\<cdot>a)) (thunks \<Delta>) (Texp e\<cdot>a)) \<sqsubseteq> Theap \<Delta> e\<cdot>a"  by (rule Theap_substitute)
     also
-    have "pathsCard (paths (substitute (FBinds \<Gamma>\<cdot>ae) (thunks \<Gamma>) (substitute (FBinds \<Delta>\<cdot>(Aheap \<Delta> e\<cdot>a)) (thunks \<Delta>) (Fexp e\<cdot>a) \<otimes>\<otimes> Fstack as S))) f|` (- domA \<Delta>) =
-          pathsCard (paths (substitute (FBinds \<Gamma>\<cdot>ae) (thunks \<Gamma>) (ftree_restr (- domA \<Delta>) (substitute (FBinds \<Delta>\<cdot>(Aheap \<Delta> e\<cdot>a)) (thunks \<Delta>) (Fexp e\<cdot>a)) \<otimes>\<otimes> Fstack as S)))"
-          by (simp add: filter_paths_conv_free_restr2 ftree_rest_substitute2[OF disj1' const_on3] ftree_restr_both  ftree_restr_noop[OF disj2'])
-    also have "ftree_restr (- domA \<Delta>) (substitute (FBinds \<Delta>\<cdot>(Aheap \<Delta> e\<cdot>a))  (thunks \<Delta>)  (Fexp e\<cdot>a)) \<sqsubseteq> Fexp (Terms.Let \<Delta> e)\<cdot>a" by (rule Fexp_Let)
+    have "pathsCard (paths (substitute (FBinds \<Gamma>\<cdot>ae) (thunks \<Gamma>) (substitute (FBinds \<Delta>\<cdot>(Aheap \<Delta> e\<cdot>a)) (thunks \<Delta>) (Texp e\<cdot>a) \<otimes>\<otimes> Fstack as S))) f|` (- domA \<Delta>) =
+          pathsCard (paths (substitute (FBinds \<Gamma>\<cdot>ae) (thunks \<Gamma>) (ttree_restr (- domA \<Delta>) (substitute (FBinds \<Delta>\<cdot>(Aheap \<Delta> e\<cdot>a)) (thunks \<Delta>) (Texp e\<cdot>a)) \<otimes>\<otimes> Fstack as S)))"
+          by (simp add: filter_paths_conv_free_restr2 ttree_rest_substitute2[OF disj1' const_on3] ttree_restr_both  ttree_restr_noop[OF disj2'])
+    also have "ttree_restr (- domA \<Delta>) (substitute (FBinds \<Delta>\<cdot>(Aheap \<Delta> e\<cdot>a))  (thunks \<Delta>)  (Texp e\<cdot>a)) \<sqsubseteq> Texp (Terms.Let \<Delta> e)\<cdot>a" by (rule Texp_Let)
     finally
     show "prognosis (Aheap \<Delta> e\<cdot>a \<squnion> ae) as a (\<Delta> @ \<Gamma>, e, S) \<sqsubseteq> cHeap \<Delta> e\<cdot>a \<squnion> prognosis ae as a (\<Gamma>, Terms.Let \<Delta> e, S)"
       by (simp add: cHeap_def del: fun_meet_simp) 
