Launchbury/FTree-Nominal-HOLCF.thy
@@ -4,9 +4,9 @@ begin
 
 (* TODO: This ssems to be unused *)
 
-instantiation ftree :: (pt) pt
+instantiation ttree :: (pt) pt
 begin
-  lift_definition permute_ftree :: "perm \<Rightarrow> 'a ftree \<Rightarrow> 'a ftree" is "\<lambda> p xss. map (\<lambda> xs. permute p xs) ` xss"
+  lift_definition permute_ttree :: "perm \<Rightarrow> 'a ttree \<Rightarrow> 'a ttree" is "\<lambda> p xss. map (\<lambda> xs. permute p xs) ` xss"
     by (auto intro: downset_mapI)
   instance by default (transfer, simp add: image_comp)+
 end
@@ -14,11 +14,11 @@ end
 lemma paths_eqvt[eqvt]: "\<pi> \<bullet> (paths t) = paths (\<pi> \<bullet> t)"
   by transfer (simp add: map_permute permute_set_eq_image)
 
-instance ftree :: (pt) cont_pt
+instance ttree :: (pt) cont_pt
 proof default
   fix p
-  show "cont (permute p :: 'a ftree \<Rightarrow> 'a ftree)"
-    by (rule ftree_contI) (transfer, auto)
+  show "cont (permute p :: 'a ttree \<Rightarrow> 'a ttree)"
+    by (rule ttree_contI) (transfer, auto)
 qed
 
 end
